\documentclass{article}
\newcommand*{\qed}{\hfill\ensuremath{\blacksquare}}
\usepackage{amsmath}
\usepackage{amssymb}

\title{Computational Linear Algebra, Assignment 1}
\author{Maya Shende}
\date{Due: February 15th, 2018}

\begin{document}
\maketitle

\begin{enumerate}
	
	\item Suppose $z_1 = a_1 + ib_1$ and $z_2 = a_2 + ib_2$. 
	\begin{enumerate}
		
		\item Prove $\overline{z_1+z_2} = \overline{z_1} + \overline{z_2}$
			Proof: 
			\begin{eqnarray*}
				\overline{z_1+z_2} &=&\overline{a_1+ib_1 + a_2+ib_2}\\
				&=& \overline{a_1+a_2+i(b_1+b_2)}\\
				&=& (a_1+a_2) - i(b_1+b_2)\\
				&=& (a_1 - ib_1) + (a_2 - ib_2)\\
				&=& \overline{a_1+ib_1} + \overline{a_2+ib_2}\\
				&=& \overline{z_1} + \overline{z_2}
			\end{eqnarray*}
			 \qed
		\item Prove $\overline{z_1-z_2} = \overline{z_1} - \overline{z_2}$
			Proof: 
			\begin{eqnarray*}
				\overline{z_1-z_2} &=&\overline{(a_1+ib_1) - (a_2+ib_2)}\\
				&=& \overline{(a_1-a_2)+i(b_1-b_2)}\\
				&=& (a_1-a_2) - i(b_1-b_2)\\
				&=& (a_1 - ib_1) - (a_2 - ib_2)\\
				&=& \overline{a_1+ib_1} - \overline{a_2+ib_2}\\
				&=& \overline{z_1} - \overline{z_2}
			\end{eqnarray*}
			 \qed
			 
		\item Prove $\overline{z_1z_2} = (\overline{z_1} )(\overline{z_2})$
			Proof: 
			\begin{eqnarray*}
				\overline{z_1z_2} &=&\overline{(a_1+ib_1) (a_2+ib_2)}\\
				&=& \overline{a_1a_2 + ia_1b_2 + ia_2b_1 - b_1b_2)}\\
				&=& \overline{((a_1a_2 - b_1b_2) + i(a_1b_2+a_2b_1))}\\
				&=& (a_1a_2 - b_1b_2) - i(a_1b_2+a_2b_1) \\
				&=& a_1a_2-b_1b_2-ia_1b_2-ia_2b_1\\
				&=& (a_1-ib_1)(a_2-ib_2)\\
				&=& (\overline{z_1})(\overline{z_2})
			\end{eqnarray*}
			 \qed

	\end{enumerate}
\end{enumerate}

\end{document}